Refactor Graph and related
Removed the N arg from node (id) which was being useless.
Rewrote and delete some auxiliary functions for graphs.

src/Graph.v
@@ -9,70 +9,74 @@ From extructures Require Import ord fset fmap.
 
 Section GraphQLGraph.
 
-  Variables (N S Vals : ordType).
+  Variables (F Vals : ordType).
 
 
   (** Field 
-      It corresponds to a field's name and list of arguments but without
-      its associated value.
+      It corresponds to an edge's label or a property's key, with a list of arguments
    **)
-  Structure fld := Field {
-                   label : S;
-                   args : {fmap S -> Vals}
+  Record fld := Field {
+                   label : F;
+                   args : {fmap F -> Vals}
                  }.
 
-
-
   
-  Definition prod_of_fld (f : fld) := let: Field l a := f in (l, a).
-  Definition fld_of_prod (p : prod S {fmap S -> Vals}) := let: (l, a) := p in Field l a.
+  Coercion label_of_fld (f : fld) := let: Field l _ := f in l.
+  Coercion fun_of_fld (f : fld) := let: Field _ a := f in a.
 
+
+  (** Packing and unpacking of graph fields, needed for canonical instances  **)
+  Definition prod_of_fld (f : fld) := let: Field l a := f in (l, a).
+  Definition fld_of_prod (p : F * {fmap F -> Vals}) := let: (l, a) := p in Field l a.
+
+  (** Cancelation lemma **)
   Lemma can_fld_of_prod : cancel prod_of_fld fld_of_prod.
   Proof. by case. Qed.
 
-  Definition fld_eqMixin := CanEqMixin can_fld_of_prod.
-  Canonical fld_eqType := EqType fld fld_eqMixin.
-  Definition fld_choiceMixin := CanChoiceMixin can_fld_of_prod.
-  Canonical fld_choiceType := ChoiceType fld fld_choiceMixin.
-  Definition fld_ordMixin := CanOrdMixin can_fld_of_prod.
-  Canonical fld_ordType := OrdType fld fld_ordMixin.
+  Canonical fld_eqType := EqType fld (CanEqMixin can_fld_of_prod).
+  Canonical fld_choiceType := ChoiceType fld (CanChoiceMixin can_fld_of_prod).
+  Canonical fld_ordType := OrdType fld (CanOrdMixin can_fld_of_prod).
   
 
 
   (** Node
-      It corresponds to a node in a graph, containing
-      an identifier, its type and its fields (as a partial mapping between
+      It corresponds to a node in a graph.
+      It contains its type and its fields (as a partial mapping between
       Fields and values).
    **)
-  Structure node := Node {
-                    id : N;
-                    type : S;
-                    fields : {fmap fld -> (Vals + (seq Vals))}
+  Record node := Node {
+                    type : F;
+                    fields : {fmap fld -> (Vals + (seq Vals))}  (* Vals could include list values? *)
                   }.
 
+  Coercion fun_of_node (n : node) := let: Node _ f := n in f.
 
-  
-  Definition prod_of_node (n : node) := let: Node i t f := n in (i, t, f).
-  Definition node_of_prod (p : N * S *  {fmap fld -> (Vals + (seq Vals)) }) :=
-    let: (i, t, f) := p in Node i t f.
+  (** Packing and unpacking of graph nodes, needed for canonical instances **)
+  Definition prod_of_node (n : node) := let: Node t f := n in (t, f).
+  Definition node_of_prod (p : F *  {fmap fld -> (Vals + (seq Vals)) }) :=
+    let: (t, f) := p in Node t f.
 
+  (** Cancelation lemma for a node **)
   Definition prod_of_nodeK : cancel prod_of_node node_of_prod.
   Proof. by case. Qed.
-  
-  Definition node_eqMixin := CanEqMixin prod_of_nodeK.
-  Canonical node_eqType := EqType node node_eqMixin.
-  Definition node_choiceMixin := CanChoiceMixin prod_of_nodeK.
-  Canonical node_choiceType := ChoiceType node node_choiceMixin.
-  Definition node_ordMixin := CanOrdMixin prod_of_nodeK.
-  Canonical node_ordType := OrdType node node_ordMixin.
-  
 
-  Definition pred_of_node (n : node) : collective_pred fld :=
-    [pred f : fld | isSome (n.(fields) f)].
+  
+  Canonical node_eqType := EqType node (CanEqMixin prod_of_nodeK).
+  Canonical node_choiceType := ChoiceType node (CanChoiceMixin prod_of_nodeK).
+  Canonical node_ordType := OrdType node (CanOrdMixin prod_of_nodeK).
+  
+  
+  Definition mem_field (n : node) f := isSome (n f).
+  
+  Definition pred_of_node (n : node) : pred_class :=
+    [eta mem_field n].
 
   Canonical node_predType := mkPredType pred_of_node.
 
-  
+
+  Lemma mem_fieldE (n : node) f : f \in n = isSome (n f).
+  Proof. done. Qed.
+
   
   (** GraphQL Graph 
       The collection of edges, and a root node 
@@ -81,51 +85,59 @@ Section GraphQLGraph.
                             root : node;
                             E : {fset node * fld * node};
                           }.
-                                    
+
+  (*
+    Record graphQLGraph := GraphQLGraph {
+           root : node;
+           nodes : {fset node};
+           E : {fset node * fld * node}
+    }
+
+    Record wfGraph := WFGraph {
+           graph : graphQLGraph;
+           _ : root \in nodes;
+           _ : forall n f v, (n, f, v) \in E -> n \in nodes /\ v \in nodes
+   }
+   *)
 
   
-
+  (** Packing and unpacking for graphs, needed for canonical instances **)
   Definition prod_of_graph (g : graphQLGraph) := let: GraphQLGraph r e := g in (r, e).
   Definition graph_of_prod (p : node * {fset node * fld * node}) :=
     let: (r, e) := p in GraphQLGraph r e.
 
+
+  (** Cancelation lemma for a graph **)
   Definition prod_of_graphK : cancel prod_of_graph graph_of_prod.
   Proof. by case. Qed.
   
-  Definition graph_eqMixin := CanEqMixin prod_of_graphK.
-  Canonical graph_eqType := EqType graphQLGraph graph_eqMixin.
-  Definition graph_choiceMixin := CanChoiceMixin prod_of_graphK.
-  Canonical graph_choiceType := ChoiceType graphQLGraph graph_choiceMixin.
-  Definition graph_ordMixin := CanOrdMixin prod_of_graphK.
-  Canonical graph_ordType := OrdType graphQLGraph graph_ordMixin.
+  Canonical graph_eqType := EqType graphQLGraph (CanEqMixin prod_of_graphK).
+  Canonical graph_choiceType := ChoiceType graphQLGraph (CanChoiceMixin prod_of_graphK).
+  Canonical graph_ordType := OrdType graphQLGraph (CanOrdMixin prod_of_graphK).
   
-  
-  Coercion label_of_fld (f : fld) := let: Field l _ := f in l.
-  Coercion fun_of_fld (f : fld) := let: Field _ a := f in a.
-
-  Coercion type_of_node (n : node) := let: Node _ t _ := n in t.
-  Coercion fun_of_node (n : node) := let: Node _ _ f := n in f.
-  
+    
     
 
   Definition fun_of_graph (g : graphQLGraph) := fun v1 f v2 => (v1, f, v2) \in (E g).
   Coercion fun_of_graph : graphQLGraph >-> Funclass.
-  
+
   Lemma graphE (g : graphQLGraph) v1 f v2 : g v1 f v2 = ((v1, f, v2) \in g.(E)).
-    Proof. done. Qed.
+  Proof. done. Qed.
+
+
     
   Coercion edges_of_graph (g : graphQLGraph) := g.(E).
 
-
-
+  
+  
 
 
 
 End GraphQLGraph.
 
 
-Arguments fld [S Vals].
-Arguments node [N S Vals].
-Arguments graphQLGraph [N S Vals].
+Arguments fld [F Vals].
+Arguments node [F Vals].
+Arguments graphQLGraph [F Vals].
 
   
